details towards more AEAD

src/tls/StreamAE.fst
@@ -22,20 +22,30 @@ open TLSConstants
 open TLSInfo
 open StreamPlain
 
-
 let gen parent i = 
   let kv = CoreCrypto.random (CoreCrypto.aeadKeySize (alg i)) in
   let iv = CoreCrypto.random (iv_length i) in
   let writer_r = new_region parent in
   if authId i then 
-    let log : ideal_log writer_r i = alloc_mref_seq writer_r Seq.createEmpty in
-    let h = ST.get() in
-    assert(0 <= max_ctr); 
-    assert(0 <= Seq.length (m_sel #writer_r #(s:seq (entry i){True}) h log));
-    let ectr: ideal_ctr writer_r i log = new_seqn writer_r 0 max_ctr log in
-    State #i #Writer #writer_r #writer_r kv iv log ectr
+    begin 
+      let log : ideal_log writer_r i = alloc_mref_seq writer_r Seq.createEmpty in
+      let h = ST.get() in
+      assert(0 <= max_seqn); 
+      assert(0 <= Seq.length (m_sel #writer_r #(s:seq (entry i){True}) h log));
+      let ectr: ideal_seqn writer_r i log = new_seqn writer_r 0 max_seqn log in
+
+      //16-09-13 can we avoid the coercion below?
+      let log : maybe_log writer_r i = to_maybe_log log in 
+      let w = State #i #Writer #writer_r #writer_r kv iv log ectr in
+
+      //16-09-13 these are now needed to prove the (authID ==> ...) postcondition
+      let h1 = ST.get() in 
+      assert(m_contains #writer_r #(s:seq (entry i){True}) (ilog w.log) h1);
+      assert(m_sel h1 (ilog w.log) == createEmpty);
+      w
+    end
   else 
-    let ectr: concrete_ctr writer_r i = m_alloc writer_r 0 in
+    let ectr: concrete_seqn writer_r i = m_alloc writer_r 0 in
     State #i #Writer #writer_r #writer_r kv iv () ectr 
 
 
@@ -44,14 +54,17 @@ let genReader parent #i w =
   if authId i
   then
     let log : ideal_log w.region i = w.log in
-    let dctr: ideal_ctr reader_r i log = new_seqn reader_r 0 max_ctr log in
+    let h = ST.get() in
+    assert(0 <= max_seqn); 
+    assert(0 <= Seq.length (m_sel #w.region #(s:seq (entry i){True}) h log));
+    let dctr: ideal_seqn reader_r i log = new_seqn reader_r 0 max_seqn log in
     State #i #Reader #reader_r #(w.region) w.key w.iv w.log dctr
-  else let dctr : concrete_ctr reader_r i = m_alloc reader_r 0 in
+  else let dctr : concrete_seqn reader_r i = m_alloc reader_r 0 in
     State #i #Reader #reader_r #(w.region) w.key w.iv () dctr
 
 let coerce parent i kv iv =
   let writer_r = new_region parent in
-  let ectr: concrete_ctr writer_r i = m_alloc writer_r 0 in
+  let ectr: concrete_seqn writer_r i = m_alloc writer_r 0 in
   State #i #Writer #writer_r #writer_r kv iv () ectr 
 
 let leak #i #role s = State.key s, State.iv s
@@ -68,7 +81,7 @@ let leak #i #role s = State.key s, State.iv s
 // we can reason about sequence-number collisions before applying it.
 let aeIV i (seqn:seqnum) (staticIV:iv i) : lbytes (iv_length i) =
   lemma_repr_bytes_values seqn;
-  max_ctr_value ();
+  max_seqn_value ();
   let extended = bytes_of_int (iv_length i) seqn in
   xor (iv_length i) extended staticIV
 
@@ -82,6 +95,7 @@ let noAD = empty_bytes
 let encrypt #i e l p =
   let ctr = ctr e.seqn in 
   m_recall ctr;
+  assume(safeId i <==> authId i); //TODO elsewhere
   let text = if safeId i then createBytes l 0z else repr i l p in
   let n = m_read ctr in
   let iv = aeIV i n e.iv in
@@ -90,9 +104,15 @@ let encrypt #i e l p =
     begin
     let ilog = ilog e.log in
     m_recall ilog;
-    let ictr: ideal_ctr e.region i ilog = e.seqn in
-    testify_seqn ictr;
+    let ictr: ideal_seqn e.region i ilog = e.seqn in
+    testify_seqn ictr; //now we know that j <= Seq.length log
+    let h = ST.get() in 
+    m_recall ilog;
+    m_recall ictr;
+    assert(m_sel h ictr <= Seq.length (m_sel h ilog)); 
     write_at_end ilog (Entry l c p); //need to extend the log first, before incrementing the seqn for monotonicity; do this only if ideal
+    let h = ST.get() in
+    assert (m_sel h ictr < Seq.length (m_sel h ilog)); 
     m_recall ictr;
     increment_seqn (fun _ -> True) ictr;
     m_recall ictr
@@ -101,6 +121,7 @@ let encrypt #i e l p =
     m_write ctr (n + 1);
   c
 
+#set-options "--z3timeout 10000"
 // decryption, idealized as a lookup at index d.seq# in the log for safe instances
 let decrypt #i d l c =
   let ctr = ctr d.seqn in 
@@ -110,7 +131,7 @@ let decrypt #i d l c =
   then 
     let ilog = ilog d.log in
     let log  = m_read ilog in
-    let ictr: ideal_ctr d.region i ilog = d.seqn in
+    let ictr: ideal_seqn d.region i ilog = d.seqn in
     let _ = testify_seqn ictr in //now we know that j <= Seq.length log
     if j < Seq.length log && matches l c (Seq.index log j) then
       begin
@@ -121,13 +142,18 @@ let decrypt #i d l c =
     else None
   else //concrete
      let iv = aeIV i j d.iv in
-     match CoreCrypto.aead_decrypt (alg i) d.key iv noAD c with
+     let o = CoreCrypto.aead_decrypt (alg i) d.key iv noAD c in 
+     match o with
      | None -> None
      | Some pr ->
        begin
-       match mk_plain i l pr with
-       | Some p -> (m_write ctr (j + 1); Some p)
-       | None   -> None
+         let a = alg i in 
+         //16-09-13  can't prove a precondition below, why?
+         assert(c = CoreCrypto.aead_encryptT a d.key iv noAD pr);
+         assert(length c = length pr + CoreCrypto.aeadTagSize a);
+         match mk_plain i l pr with
+         | Some p -> (m_write ctr (j + 1); Some p)
+         | None   -> None
        end
 
 
